QuantifierLean/Lemmas2_1.lean
@@ -1,9 +1,0 @@
-
-import Mathlib.Tactic
-import QuantifierLean.Definitions2
-import QuantifierLean.Lemmas2
-
-import Mathlib.Data.Vector.Snoc
-import Mathlib.Logic.Basic
-
-open Mathlib
